src/examples/Test.FnType.fst
@@ -1,0 +1,10 @@
+module Test.FnType
+#lang-pulse
+open Pulse
+
+fn test
+  (frame : slprop)
+  (fn f (x : int) requires frame ensures frame)
+  requires frame
+  ensures frame
+{ f 0; }
