src/lib/kuiper/Kuiper.Kernel.Par.fst
@@ -6,8 +6,8 @@ open Pulse.Lib.ConditionVar
 
 fn par (#preL: slprop) #postL #preR #postR (vis: visibility) #l0 (l: loc_id)
   {| is_send_across vis preL, is_send_across vis postL |}
-  (f:unit -> stt unit (loc l ** preL) (fun _ -> loc l ** postL))
-  (g:unit -> stt unit preR (fun _ -> postR))
+  (fn f () requires loc l ** preL ensures loc l ** postL)
+  (fn g () requires preR ensures postR)
   preserves loc l0 ** pure (vis l0 == vis l)
   requires preL ** preR
   ensures postL ** postR
