src/lib/poly/Kuiper.Poly.Softmax.fsti
@@ -26,16 +26,15 @@ let softmax_real (s:Seq.seq real { Seq.length s > 0 }) =
 
 unfold
 type softmax_gpu_ty (et : Type0) {| floating et, real_like et, floating_real_like et |} =
-  (#lena : szp { lena < max_threads }) ->
-  (a : gpu_array et lena { is_global_array a }) ->
-  (#va : erased (seq et)) ->
-  (#ra : erased (seq real) { Seq.length ra == SizeT.v lena /\ va %~ ra /\ lena > 0 }) ->
-  stt unit
-  (requires
+  fn (#lena : szp { lena < max_threads })
+     (a : gpu_array et lena { is_global_array a })
+     (#va : erased (seq et))
+     (#ra : erased (seq real) { Seq.length ra == SizeT.v lena /\ va %~ ra /\ lena > 0 })
+  requires
     cpu **
     (on gpu_loc (a |-> va) **
-     pure (lena <= max_blocks)))
-  (ensures fun _ ->
+     pure (lena <= max_blocks))
+  ensures (
     cpu **
      (exists* (v':seq et). on gpu_loc (a |-> v') **
         pure (v' %~ softmax_real ra)))
@@ -46,16 +45,15 @@ val softmax_gpu (#et:Type0) {| floating et, real_like et, floating_real_like et 
 
 unfold
 type softmax_ty (et : Type0) {| floating et, real_like et |} =
-  (#lena : szp { lena < max_threads }) ->
-  (a : Vec.lvec et lena) ->
-  (#va : erased (seq et)) ->
-  (#ra : erased (seq real) { Seq.length ra == SizeT.v lena /\ va %~ ra /\ lena > 0 }) ->
-  stt unit
-  (requires
+  fn (#lena : szp { lena < max_threads })
+     (a : Vec.lvec et lena)
+     (#va : erased (seq et))
+     (#ra : erased (seq real) { Seq.length ra == SizeT.v lena /\ va %~ ra /\ lena > 0 })
+  requires
     cpu **
     (a |-> va **
-     pure (lena <= max_blocks)))
-  (ensures fun _ ->
+     pure (lena <= max_blocks))
+  ensures (
     cpu **
     (exists* (v':seq et). a |-> v' **
         pure (v' %~ softmax_real ra)))
